{
 "cells": [
  {
   "cell_type": "markdown",
   "metadata": {},
   "source": [
    "Polynomial $A(x) = \\sum_{j=0}^{n-1} a_j x^j$\n",
    "\n",
    "let coeffs $A = (a_0,...,a_{n-1})$.\n",
    "\n",
    "that $k=0,...,n-1$\n",
    "$$\n",
    "\\begin{align}\n",
    "\\text{DFT}(A) &= (\\sum_{j=0}^{n-1} a_j e^{-\\frac{2\\pi i}{n} jk},...)_k \\\\\n",
    "    &= (A(\\omega_n^k),...)_k,\\ \\ \\  \\omega_n^k = \\exp(-\\frac{2\\pi i}{n} k)\n",
    "\\end{align}\n",
    "$$\n",
    "\n",
    "then consider convolution, or multiplication of $A(x)$ and $B(x)$. we wanna know coeffs of  $(A*B)(x) = A(x)B(x)$.\n",
    "\n",
    "for simplicity write $F=DFT$, notice that, $F(A) = (A(\\omega_n^k))_k$, that\n",
    "\n",
    "$$\n",
    "\\begin{align}\n",
    "    F(A*B)  &= ((A*B)(\\omega_n^k))_k = (A(\\omega_n^k)B(\\omega_n^k))_k = F(A)\\cdot  F(B) \\\\\n",
    "    A*B &= F^{-1}[F(A)\\cdot  F(B)]\n",
    "\\end{align}\n",
    "$$\n",
    "\n",
    "so next we need is to compute $F, F^{-1}$ in $O(n\\log n)$\n",
    "\n",
    "Before continue, note the lemmas\n",
    "\n",
    "$$\n",
    "\\begin{align}\n",
    "    \\omega_{dn}^{dk} = \\omega_n^k, n,k,d \\geq 0 \\\\\n",
    "    \\omega_n^{n/2} = \\omega_2^1 = -1,  n>0 \\\\\n",
    "    (\\omega_n^{k+n/2})^2=(\\omega_n^k)^2=\\omega_{n/2}^k, n>0, \\text{even} \\\\\n",
    "    \\omega_n^{k+n/2} = -\\omega_n^k, n\\geq 0\n",
    "\\end{align}\n",
    "$$\n",
    "\n",
    "then by separate odd,even, i.e. $A(x) = A_0(x^2) + xA_1(x^2)$. combine above lemmas, get\n",
    "\n",
    "$$\n",
    "\\begin{align}\n",
    "    A(\\omega_n^k) = A_0(\\omega_{n/2}^k) + \\omega_n^k A_1(\\omega_{n/2}^k), 0\\leq k < n/2 \\\\\n",
    "    A(\\omega_n^{k+n/2}) = A_0(\\omega_{n/2}^k) - \\omega_n^k A_1(\\omega_{n/2}^k), k+n/2 \\geq n/2\n",
    "\\end{align}\n",
    "$$\n",
    "\n",
    "Thus, by divide and conquer solved. what about $F^{-1}$. notice that matrix form\n",
    "\n",
    "$$\n",
    "\\begin{align}\n",
    "    y=F(A) = W a \\\\\n",
    "    w_{k,j} = \\omega_n^{kj}, k,j=0,...n-1\\\\\n",
    "    a = F^{-1}(y) = W^{-1}y\n",
    "\\end{align}\n",
    "$$\n",
    "\n",
    "by the special form of $W$\n",
    "$$\n",
    "\\begin{align}\n",
    "    W^{-1} = \\frac{1}{n} \\bar{W}\\\\\n",
    "    v_{kj} = \\frac{1}{n} \\bar{w_n} ^{kj}\n",
    "\\end{align}\n",
    "$$\n",
    "\n",
    "So, just conjugate and divided by $n$. then same method sovlable."
   ]
  },
  {
   "cell_type": "markdown",
   "metadata": {},
   "source": [
    "### NTT\n",
    "\n",
    "let $\\alpha$ replace $\\omega_n$ in integer field.\n",
    "\n",
    "DFT require\n",
    "$$\n",
    "\\begin{align}\n",
    "    \\sum_{j=0}^{n-1} \\alpha^{kj} = 0, k=1,...,n-1\n",
    "\\end{align}\n",
    "$$\n",
    "and $\\alpha^n=1, \\alpha^k \\neq 1, k=1,...,n-1$ is sufficient\n",
    "\n",
    "if $n$ is power of $2$, $\\alpha^{n/2} = -1$ is sufficient\n",
    "\n",
    "if we get the $\\alpha$ on $Z_p$, then $p=c2^k+1$, that $\\alpha^c$ can be the $\\alpha'$ to express conv length $\\leq 2^{k-1}$\n",
    "\n",
    "For in place NTT, leaves' addr. are bit-reversed. (NEED rigorous proof)\n",
    "\n",
    "and if for $F^{-1}$, one way is calc $\\alpha^{-1}$, for each iter. Here is another way. Notice the matrix form. suppose $a$ divided by $n$, then we reverse $[a_1,...,a_{n-1}]$. by the fact $\\alpha^{k(n-j)} = \\alpha^{-kj}$, thus result is exactly $F^{-1}$. \n",
    "\n",
    "#### inverse\n",
    "\n",
    "we wanna know $BA \\equiv 1 (\\mod x^n)$. by the step that double $B$'s size, with init $B_0=1/A_0$. wlog write $B_1$ repre. $B_n$, $B_2$ repre. $B_{2n}$. that\n",
    "$$\n",
    "\\begin{align}\n",
    "    & (B_1 A - 1)^2 \\equiv 0 (\\mod x^2) \\\\\n",
    "    \\Rightarrow  & B_2 = 2B_1 - B_1^2 A (\\mod x^2)\n",
    "\\end{align}\n",
    "$$\n",
    "note, in impl. $B_1^2A$ has $B_1(\\mod x)$ part in there since $B_1A \\equiv 1(\\mod x)$. aka, $(\\mod x)$ part remain $B_1$, actually, we only need modify the higher order part, $-B_1^2 A ([x\\leq..<x^2])$ \n",
    "\n",
    "#### sqrt\n",
    "\n",
    "also, the double size technique\n",
    "$$\n",
    "\\begin{align}\n",
    "    & (B_1^2 - A)^2 \\equiv 0 (\\mod x^2) \\\\\n",
    "    \\Rightarrow  & B_2 = \\frac{1}{2} [B_1 + A B_1^{-1}](\\mod x^2)\n",
    "\\end{align}\n",
    "$$\n",
    "again, notice the old part $B_1$ shall remain, we can only modify new part in impl. and careful $B_0^2=A_0$ when $\\neq 1$\n",
    "\n",
    "#### log\n",
    "\n",
    "$\\log P = \\int \\frac{P'}{P}$\n",
    "\n",
    "#### exponent\n",
    "\n",
    "double step, $B_2 = B_1(1 + A - \\log B_1)$"
   ]
  },
  {
   "cell_type": "markdown",
   "metadata": {},
   "source": [
    "### FWHT(FHT)\n",
    "\n",
    "Hadamard transform, def, with $H_0 = 1$\n",
    "$$\n",
    "\\begin{align}\n",
    "    H_m = \\frac{1}{\\sqrt{2}} \\begin{bmatrix} H_{m-1} & H_{m-1} \\\\ H_{m-1} & -H_{m-1} \\end{bmatrix} \\\\\n",
    "    (H_m)_{i,j} = \\frac{1}{2^{m/2}} (-1)^{\\langle i, j \\rangle_b}\n",
    "\\end{align}\n",
    "$$\n",
    "where $i,j= 0,1,..,2^m-1$ and $\\langle .,.\\rangle_b$ is bitwise dot product, aka\n",
    "```\n",
    "__builtin_popcount(i&j)\n",
    "```\n",
    "\n",
    "when do fwht, don't need bit reversal and generator. besides, there is good property $H_m^2= I$.\n",
    "One can easy show $H_1^2 = I$ by direct compute or quantum tech. $H_1 = |+\\rangle \\langle 0| + |-\\rangle \\langle 1| $. then by induction. $H_m = H_1 \\otimes H_{m-1}$. that $H_m^2 = H_1^2 \\otimes H_{m-1}^2 = I$. which means we can do $H^{-1}$ by direct do $H$ !\n",
    "\n",
    "note in impl. we often omit $2^{n/2}$, that use $H' = 2^{n/2}H$. so when do inverse, we need divide by $2^n$.\n",
    "\n",
    "still, we can do multiply by $A*B = H^{-1} [H(A) \\cdot H(B)]$. note $\\cdot$ is element-wise mult.\n",
    "\n",
    "also, suprisingly, for solving equation $A*B = C$, if we put $H$ on each side, that\n",
    "\n",
    "$H(A) \\cdot H(B) = H(C)$, since $\\cdot$ is element-wised, thus we can get $A = H^{-1} [H(C) / H(B)]$, element-wise.\n",
    "\n",
    "Note. for $\\sum_i B_i = 0$, aka, not linear indep. the solution may has many, notice that $R = (1,1,...,1)$, that $R*B = 0$. e.g. agc034f.\n",
    "\n",
    "so we can minus arbitral still solution, but according specific condition, we can get the right one."
   ]
  },
  {
   "cell_type": "markdown",
   "metadata": {},
   "source": [
    "### useful links\n",
    "\n",
    "https://cp-algorithms.com/algebra/fft.html\n",
    "\n",
    "https://cp-algorithms.com/algebra/polynomial.html#toc-tgt-4\n",
    "\n",
    "https://en.wikipedia.org/wiki/Discrete_Fourier_transform#Polynomial_multiplication\n",
    "\n",
    "https://en.wikipedia.org/wiki/Discrete_Fourier_transform_(general)\n",
    "\n",
    "https://codeforces.com/blog/entry/43499\n",
    "\n",
    "https://codeforces.com/blog/entry/48798\n",
    "\n",
    "https://crypto.stanford.edu/pbc/notes/numbertheory/gen.html\n",
    "\n",
    "https://csacademy.com/blog/fast-fourier-transform-and-variations-of-it"
   ]
  },
  {
   "cell_type": "code",
   "execution_count": null,
   "metadata": {},
   "outputs": [],
   "source": []
  }
 ],
 "metadata": {
  "kernelspec": {
   "display_name": "Python 3",
   "language": "python",
   "name": "python3"
  },
  "language_info": {
   "codemirror_mode": {
    "name": "ipython",
    "version": 3
   },
   "file_extension": ".py",
   "mimetype": "text/x-python",
   "name": "python",
   "nbconvert_exporter": "python",
   "pygments_lexer": "ipython3",
   "version": "3.7.2"
  }
 },
 "nbformat": 4,
 "nbformat_minor": 2
}
